\documentclass{article}
\usepackage[pdftex]{graphicx}
\usepackage{rotating}
\usepackage{amsmath}
\usepackage{authblk}
\usepackage{float}
\usepackage{bm}
\usepackage{multirow}
\usepackage{fullpage}
\usepackage{Sweave}
\usepackage{pdflscape}
\usepackage{amsmath}   
\usepackage{amssymb}
\usepackage{wasysym}
\usepackage{ctable}
\newcommand{\fg}[3]{\begin{figure}[htbp]%
        \leavevmode%
        \centerline{\includegraphics{#1}}%
        \caption{#3}%
        \label{#2}%
        \end{figure}}
%\fgh{basefilename}{label}{caption}{short caption for TOC}
\newcommand{\fgh}[4]{\begin{figure}[htbp]%
        \leavevmode%
        \centerline{\includegraphics{#1}}%
        \caption[#4]{#3}%
        \label{#2}%
        \end{figure}}
\begin{document} 
\input{CPH687Homework4-concordance}


\title{CPH687 Homework 4}
%\author[1]{\small{Bruce Barber}}
\author{\small{Meng Lu}}

\affil{\footnotesize{GIDP Statistics \\ Email: menglu@email.arizona.edu}}
%\affil[2]{\footnotesize{Department of Pediatric, The University of Arizona}}
%\affil[2]{\footnotesize{Statistical Consulting Laboratory \\ email: zlu@arizona.edu}}

\maketitle
\section{Problem 1}
Question: \\ 
Let $y_i$ have mean $\mu$ and variance $\sigma^2$, which are
scalars. Find the expection of the estimator of $\sigma^2$
\begin{align*}
  &S^2=\frac{1}{n-1}\sum_{i=1}^{n}(y_i-\bar{y})^2
  .
  \end{align*}
using matrix notations $\bm{y_{n\times
    1}}=(y_1,y_2,\cdots,y_n)^{\prime}$ and $\bar{y}=\bm{1_n^{\prime}y}/n$\\     
Solution:\\
\begin{align*}
  S^2&=\frac{1}{n-1}\sum_{i=1}^{n}(y_i-\bar{y})^2\\
  &=\frac{1}{n-1}(\sum_{i=1}^{n}y_i^2-n(\bar{y})^2)\\
  E(S^2)&=\frac{1}{n-1}(\sum_{i=1}^{n}E(y_i^2)-nE(\bar{y}^2))\\
  &=\frac{1}{n-1}(\sum_{i=1}^{n}(Var(y_i)+(E(y_i))^2)-n(Var(\bar)+(E(\bar{y}))^2))\\
  &=\frac{1}{n-1}(n\sigma^2+n\mu^2-\sigma^2-n\mu^2)\\
  &=\sigma^2 
  .
  \end{align*}
                
\section{Problem 2}
Question:\\ 
Let $\bm{y} \sim N(\bm{\mu},\bm{\Sigma})$ where $\Sigma$ is
p.d. Verify that the MGF of $\bm{y}$ is 
\begin{align*}
  &M_{\bm{y}}(\bm{t})=exp(\bm{t^{\prime}\mu}+\frac{1}{2}\bm{t^{\prime}\Sigma
  t})
.
\end{align*}
Solution:\\
\begin{align*}
  M_{\bm{y}}(\bm{t})&=E(e^{\bm{t^{\prime}y}})\\
  &=C\int_{-\infty}^{\infty}e^{\bm{t^{\prime}y}}e^{-\frac{1}{2}\bm{(y-\mu)^{\prime}}\bm{\Sigma^{-1}(y-\mu)}}\,d\bm{y}\\
  C&=\frac{1}{(2\pi)^{-n/2}}|\bm{\Sigma}|^(-1/2)\\
  &=\int_{-\infty}^{\infty}e^{-\frac{1}{2}\bm{((y-\mu)^{\prime}\Sigma^{-1}(y-\mu)-2t^{\prime}y)}}\,d\bm{y}\\
 \bm{(y-\mu)^{\prime}\Sigma^{-1}(y-\mu)}-2\bm{t^{\prime}y}&=\bm{y^{\prime}\Sigma^{-1}y}-2\bm{y^{\prime}\Sigma^{-1}\mu+\mu^{\prime}\Sigma^{-1}\mu-2t^{\prime}y}\\
  &=\bm{y^{\prime}\Sigma^{-1}y-2y^{\prime}\Sigma^{-1}\mu+\mu^{\prime}\Sigma^{-1}\mu-2y^{\prime}\Sigma^{-1}\Sigma
  t}\\
  &=\bm{y^{\prime}\Sigma^{-1}y-2y^{\prime}\Sigma^{-1}(\mu+\Sigma t)+\mu^{\prime}\Sigma^{-1}\mu}\\
  &=\bm{[y-(\mu+\Sigma t)]^{\prime}\Sigma^{-1}[y-(\mu+\Sigma
  t)]-(\mu+\Sigma t)^{\prime}\Sigma^{-1}(\mu+\Sigma t)+\mu^{\prime}\Sigma^{-1}\mu}\\
  &=\bm{[y-(\mu+\Sigma t)]^{\prime}\Sigma^{-1}[y-(\mu+\Sigma
  t)]-(2\mu^{\prime}t+t^{\prime}\Sigma t)}\\
  &=\bm{[y-(\mu+\Sigma t)]^{\prime}\Sigma^{-1}[y-(\mu+\Sigma
  t)]-(2t^{\prime}mu+t^{\prime}\Sigma t)}\\
  \therefore M_{\bm{y}}(\bm{t})&=C\int_{-\infty}^{\infty}e^{\bm{([y-(\mu+\Sigma t)]^{\prime}\Sigma^{-1}[y-(\mu+\Sigma
  t)]-(2t^{\prime}mu+t^{\prime}\Sigma t))}}\,d\bm{y}\\
&=e^{\bm{t^{\prime}\mu}+\frac{1}{2}\bm{t^{\prime}\Sigma t}}C\int_{-\infty}^{\infty}e^{-\frac{1}{2}\bm{([y-(\mu+\Sigma t)]^{\prime}\Sigma^{-1}[y-(\mu+\Sigma
  t)])}}\,d\bm{y}\\
&=e^{\bm{t^{\prime}\mu}+\frac{1}{2}\bm{t^{\prime}\Sigma t}}
  .
  \end{align*}
       
         
                   
\section{Problem 3}
Question:\\
Let $\bm{A_{r \times n}}$ be a matrix of constants. Verify that
$\bm{Ay} \sim N(\bm{A\mu},\bm{A\Sigma A^{\prime}})$.\\     
Solution:\\
\begin{align*}
  E(\bm{Ay})&=\bm{A}E(\bm{y})=\bm{A\mu}\\
  Var(\bm{Ay})&=\bm{A}Var(\bm{y})\bm{A^{\prime}}=\bm{A\Sigma A^{\prime}}\\
  f(\bm{y}|\bm{\mu}, \bm{\Sigma})&=\frac{1}{(2\pi)^{n/2}|\bm{\Sigma}|^{-1/2}}exp[-\frac{1}{2}\bm{(y-\mu)^{\prime}\Sigma^{-1}(y-\mu)}]\\
  &\bm{x}=\bm{Ay}\rightarrow \bm{y}=\bm{A^{-1}x}\\
  f(\bm{A^{-1}x}|\bm{\mu}, \bm{\Sigma})&=\frac{1}{(2\pi)^{n/2}|\bm{A\Sigma A^{\prime}}|^{-1/2}}exp[-\frac{1}{2}\bm{(A^{-1}x-\mu)^{\prime}\Sigma^{-1}(A^{-1}x-\mu)}]\\
  &=\frac{1}{(2\pi)^{n/2}|\bm{A\Sigma A^{\prime}}|^{-1/2}}exp[-\frac{1}{2}\bm{(A^{-1}x-A^{-1}A\mu)^{\prime}\Sigma^{-1}(A^{-1}x-A^{-1}A\mu)}]\\
  &=\frac{1}{(2\pi)^{n/2}|\bm{A\Sigma A^{\prime}}|^{-1/2}}exp[-\frac{1}{2}\bm{(A^{-1}(x-A\mu))^{\prime}\Sigma^{-1}A^{-1}(x-A\mu)}]\\
  &=\frac{1}{(2\pi)^{n/2}}|\bm{A\Sigma A^{\prime}}|^{-1/2}exp[-\frac{1}{2}\bm{(x-A\mu)^{\prime}(A\Sigma A^{\prime})^{-1}(x-A\mu)}]\\
  \therefore &\bm{Ay} \sim N(\bm{A\mu},\bm{A\Sigma A^{\prime}})
  .
  \end{align*}
       

         
\section{Problem 4}
Question:\\
If $\bm{X}$ and $\bm{Y}$ are n-dimensional vectors with independent
multivariate normal distributions, prove that $a\bm{X}+b\bm{Y}$ is
also multivariate normal.\\
Solution:\\
\begin{align*}
  M_{a\bm{X}+b\bm{Y}}(\bm{t})&=E(e^{\bm{t^{\prime}}(a\bm{X}+b\bm{Y})})\\
  &=E(e^{a\bm{t^{\prime}X}}e^{b\bm{t^{\prime}Y}})\\
  \because &\bm{X} \text{ and }\bm{Y} \text{ are n-dimensional vectors with
    independent multivariate normal distributions}\\
  \therefore M_{a\bm{X}+b\bm{Y}}(\bm{t})&=E(e^{a\bm{t^{\prime}X}}e^{b\bm{t^{\prime}Y}})\\
  &=E(e^{a\bm{t^{\prime}X}})E(e^{b\bm{t^{\prime}Y}})\\
  &=exp(a\bm{t^{\prime}\mu_X}+\frac{1}{2}a^2\bm{t^{\prime}\Sigma_Xt}) exp(b\bm{t^{\prime}\mu_Y}+\frac{1}{2}b^2\bm{t^{\prime}\Sigma_Yt})\\
  &=exp(\bm{t^{\prime}}(a\bm{\mu_X}+b\bm{\mu_Y})+\frac{1}{2}\bm{t^{\prime}}(a^2\bm{\Sigma_X}+b^2\bm{\Sigma_Y}))\\
  \therefore &a\bm{X}+b\bm{Y} \text{ is also multivariate normal with
    mean }a\bm{\mu_X}+b\bm{\mu_Y}\text{ and variance }a^2\bm{\Sigma_X}+b^2\bm{\Sigma_Y}
  .
  \end{align*}


\section{Problem 5}
Question:\\
If $\bm{Y} \sim N_2(\bm{0},\bm{\Sigma})$, where
$\bm{\Sigma}=(\sigma_{ij})$, prove that
\begin{align*}
  &(\bm{Y^{\prime}\Sigma^{-1}Y}-\frac{Y_1^2}{\sigma_{11}}) \sim \chi_1^2
  .
  \end{align*}

Solution:\\
\begin{align*}
  \bm{Y^{\prime}\Sigma^{-1}Y}&=\bm{Y^{\prime}\Sigma^{-1/2}\Sigma^{-1/2}Y}\\
  &=\bm{(\Sigma^{-1/2}Y)^{\prime}\Sigma^{-1/2}Y}\\
  \text{Let }\bm{Z}=\bm{\Sigma^{-1/2}Y}\\
  Var(\bm{Z})&=I_2\\
  \text{From the Problem 3, we know that }\bm{Z} \sim N_2(\bm{0,I})\\
  \therefore (\bm{Z^{\prime}Z}-\frac{Y_1^2}{\sigma_{11}}) \sim \chi_1^2
  .
  \end{align*}
\end{document}
